update e11 notes

uw-cse-505/e11/E11_Progress.v
@@ -1,25 +1,34 @@
 Require Import List.
 Require Import String.
+Require Import ZArith.
 Open Scope string_scope.
 
 Definition var := string.
 
 Inductive Expr : Set :=
+| Bool : bool -> Expr
+| Int : Z -> Expr
 | Var : var -> Expr
 | App : Expr -> Expr -> Expr
 | Lam : var -> Expr -> Expr.
 
+Notation "'B' b" := (Bool b) (at level 48).
+Notation "'I' i" := (Int i) (at level 48).
 Notation "'V' x" := (Var x) (at level 48).
 Notation "e1 @ e2" := (App e1 e2) (at level 49).
 Notation "\ x , t" := (Lam x t) (at level 50).
 
 Check (\"x", \"y", V"x").
-Check (\"x", \"y", V"y").
+Check (\"x", \"y", I 5).
 Check ((\"x", V"x" @ V"x") @ (\"x", V"x" @ V"x")).
 
 (* e1[e2/x] = e3 *)
 Inductive Subst : Expr -> Expr -> var ->
                   Expr -> Prop :=
+| SubstBool : forall b e x,
+  Subst (B b) e x (B b)
+| SubstInt : forall i e x,
+  Subst (I i) e x (I i)
 | SubstVar_same : forall e x,
   Subst (V x) e x e
 | SubstVar_diff : forall e x1 x2,
@@ -116,6 +125,8 @@ Lemma Subst_det:
   e3 = e3'.
 Proof.
   induction 1; intros.
+  { inversion H; auto. }
+  { inversion H; auto. }
   { inversion H; subst; auto.
     congruence.
   }
@@ -294,3 +305,143 @@ Proof.
   }
 Qed.
 
+(* ----------- *)
+
+Inductive Value : Expr -> Prop :=
+| VBool : forall b,
+  Value (B b)
+| VInt : forall i,
+  Value (I i)
+| VLam : forall x e,
+  Value (\x, e).
+
+Inductive Typ :=
+| TBool : Typ
+| TInt : Typ
+| TFun : Typ -> Typ -> Typ.
+
+Notation "t1 ~> t2" := (TFun t1 t2) (at level 52).
+
+Definition Env := var -> option Typ.
+
+Definition Empty : Env := fun _ => None.
+
+Definition extend (env: Env) x t :=
+  fun y => if string_dec x y then Some t else env y.
+
+Inductive WellTyped : Env -> Expr -> Typ -> Prop :=
+| WTBool : forall env b,
+  WellTyped env (B b) TBool
+| WTInt : forall env i,
+  WellTyped env (I i) TInt
+| WTVar : forall env x t,
+  env x = Some t ->
+  WellTyped env (V x) t
+| WTLam : forall env x e t1 t2,
+  WellTyped (extend env x t1) e t2 ->
+  WellTyped env (\x, e) (t1 ~> t2)
+| WTApp : forall env e1 e2 t1 t2,
+  WellTyped env e1 (t1 ~> t2) ->
+  WellTyped env e2 t1 ->
+  WellTyped env (e1 @ e2) t2.
+
+Lemma test_WT_1:
+  WellTyped Empty
+    ((\"x", V"x") @ (\"y", V"y"))
+    (TInt ~> TInt).
+Proof.
+  econstructor.
+  { constructor. constructor. reflexivity. }
+  { constructor. constructor. reflexivity. }
+Qed.
+
+Lemma test_WT_2:
+  WellTyped Empty
+    ((\"x", V"x") @ (\"y", V"y"))
+    (TBool ~> TBool).
+Proof.
+  econstructor.
+  { constructor. constructor. reflexivity. }
+  { constructor. constructor. reflexivity. }
+Qed.
+
+Lemma canon_bool:
+  forall e,
+  Value e ->
+  WellTyped Empty e TBool ->
+  exists b, e = B b.
+Proof.
+  intros. inversion H.
+  { eauto. }
+  { subst. inversion H0. }
+  { subst. inversion H0. }
+Qed.
+
+Lemma canon_int:
+  forall e,
+  Value e ->
+  WellTyped Empty e TInt ->
+  exists i, e = I i.
+Proof.
+  intros. inversion H.
+  { subst. inversion H0. }
+  { eauto. }
+  { subst. inversion H0. }
+Qed.
+
+Lemma cannon_lam:
+  forall e t1 t2,
+  Value e ->
+  WellTyped Empty e (t1 ~> t2) ->
+  exists x, exists e', e = \x, e'.
+Proof.
+  intros. inversion H.
+  { subst. inversion H0. }
+  { subst. inversion H0. }
+  { eauto. }
+Qed.
+
+Lemma Subst_exists:
+  forall e1 e2 x,
+  exists e3, Subst e1 e2 x e3.
+Proof.
+  intros. induction e1.
+  { econstructor. constructor. }
+  { econstructor. constructor. }
+  { destruct (string_dec v x).
+    { subst. econstructor. constructor. }
+    { econstructor. constructor. assumption. }
+  }
+  { firstorder. econstructor. constructor.
+    { eassumption. }
+    { eassumption. }
+  }
+  { destruct (string_dec v x).
+    { subst. econstructor. constructor. }
+    { firstorder. econstructor. constructor.
+      { assumption. }
+      { eassumption. }
+    }
+  }
+Qed.
+
+Lemma progress:
+  forall env e t,
+  env = Empty ->
+  WellTyped env e t ->
+  ((exists e', e --> e') \/ Value e).
+Proof.
+  intros. induction H0.
+  { right. constructor. }
+  { right. constructor. }
+  { subst. discriminate. }
+  { right. constructor. }
+  { subst. destruct IHWellTyped1.
+    { reflexivity. }
+    { destruct H. left. econstructor. left. eassumption. }
+    { left. eapply cannon_lam in H.
+      { destruct H. destruct H. subst. destruct (Subst_exists x0 e2 x). econstructor. right. eassumption. }
+      { eassumption. }
+    }
+  }
+Qed.
